Name: ____________________ Student number:_____________

MAT 186 Quiz 8

1. Evaluate the following limit:

AB3 CF6 CS13

$$\lim_{x\to\infty}\frac{x^{2}-\ln(2/x)}{3x^{2}+2x}$$

The limit is of the form $\infty/\infty$, so L'Hopital is probably the way to go. Ideally, you should simplify first:

$$\begin{array} { r l } & { \operatorname* { l i m } _ { x \to \infty } \frac { x ^ { 2 } - \ln ( 2 / x ) } { 3 x ^ { 2 } + 2 x } = \operatorname* { l i m } _ { x \to \infty } \frac { x ^ { 2 } - \ln 2 + \ln x } { 3 x ^ { 2 } + 2 x } } \\ & { \quad \stackrel { L \prime H } { \cong } \operatorname* { l i m } _ { x \to \infty } \frac { 2 x - 0 + 1 / x } { 6 x + 2 } } \\ & { \quad = \operatorname* { l i m } _ { x \to \infty } \frac { 2 + 1 / x ^ { 2 } } { 6 + 2 / x } } \\ & { \quad = 1 / 3 } \end{array}$$

2. Another fun limit:

$$\operatorname* { l i m } _ { \theta \to ( \pi / 2 ) ^ { - } } (  t a n  \theta ) ^ { \cos \theta }$$

This limit is of the form $\infty^{0}$, so L'Hopital's rule applies.

$$L=\operatorname* { l i m } _{\theta \to ( \pi / 2 ) ^ { - } } ( \tan \theta ) ^ { \cos \theta }$$

$$\begin{array} { r l } & { \ln L = \operatorname* { l i m } _ { \theta \to ( \pi / 2 ) ^ { - } } \cos \theta \ln ( \tan \theta ) } \\ & { = \operatorname* { l i m } _ { \theta \to ( \pi / 2 ) ^ { - } } \frac { \ln ( \tan \theta ) } { \left( \frac { 1 } { \cos \theta } \right) } } \\ & { \stackrel { L ^ { \prime \prime } H } { \cong } \operatorname* { l i m } _ { \theta \to ( \pi / 2 ) ^ { - } } \frac { \left( \frac { 1 } { \tan \theta } \cdot  \sec ^ { 2 } \theta \right) } { \left( \frac { - 1 } { \cos ^ { 2 } \theta } \cdot  ( - \sin \theta ) \right) } } \\ & { = \operatorname* { l i m } _ { \theta \to ( \pi / 2 ) ^ { - } } \frac { \cos \theta } { \sin ^ { 2 } \theta } = 0 } \\ & { \therefore L = e ^ { 0 } = 1 } \end{array}$$

<table><tr><td>AB3</td><td>AB5</td><td>CF6</td><td>CS13</td><td>CS14</td></tr></table>


Continued on back.

---

AB8 CF18 CF19

3. For the function $f(x)=6x-2$, over the interval $[-2,2]$, find the area under the graph using Riemann sums.

For the Riemann sum, we take $\Delta x=\frac{2-(-2)}{n}=\frac{4}{n}$.

Therefore, $x_{k}=a+k\Delta x=-2+{\frac {4}{n}}k$.

It is easiest to use a right-hand sum:

$$\begin{array} { r l } & { \int _ { - 2 } ^ { 2 } 6 x - 2 \, d x = \operatorname* { l i m } _ { n \to \infty } \sum _ { k = 1 } ^ { n } ( 6 x _ { k } ^ { * } - 2 ) ( \Delta x ) } \\ & { = \operatorname* { l i m } _ { n \to \infty } \sum _ { k = 1 } ^ { n } \left( 6 \left( - 2 + \frac { 4 } { n } k \right) - 2 \right) \left( \frac { 4 } { n } \right) } \\ & { = \operatorname* { l i m } _ { n \to \infty } \sum _ { k = 1 } ^ { n } \left( - 1 4 + \frac { 2 4 } { n } k \right) \left( \frac { 4 } { n } \right) } \\ & { = \operatorname* { l i m } _ { n \to \infty } \sum _ { k = 1 } ^ { n } \left( - \frac { 5 6 } { n } + \frac { 9 6 } { n ^ { 2 } } k \right) } \\ & { = \operatorname* { l i m } _ { n \to \infty } \left( \sum _ { k = 1 } ^ { n } \left( - \frac { 5 6 } { n } \right) + \sum _ { k = 1 } ^ { n } \left( \frac { 9 6 } { n ^ { 2 } } k \right) \right) } \\ & { = \operatorname* { l i m } _ { n \to \infty } \left( - 5 6 + \frac { 9 6 } { n ^ { 2 } } \cdot  \frac { n ( n + 1 ) } { 2 } \right) } \\ & { = - 5 6 + 4 8 } \\ & { = - 8 } \end{array}$$

4. Verify your answer from question 3, using antiderivatives.

$$\begin{array} { r l } & { \int _ { - 2 } ^ { 2 } 6 x - 2 \, d x = ( 3 x ^ { 2 } - 2 x ) _ { - 2 } ^ { 2 } } \\ &  & { = ( 1 2 - 4 ) - ( 1 2 + 4 ) } \\ &  & { = - 8 } \end{array}$$

CF16

